v2/LscV2/Core/ContractM.lean
@@ -1,4 +1,4 @@
-import LscV2.AST
+import LscV2.Lang.AST
 import LscV2.Arithmetic
 
 namespace LscV2
