v2/LscV2/Lib/Wei.lean
@@ -1,6 +1,3 @@
-import LscV2.Lib.Wei.Type
-import LscV2.Lib.Wei.Arith
-import LscV2.Lib.Wei.Expr
-import LscV2.Lib.Wei.Checks
+import LscV2.Lib.Wei.Syntax
 import LscV2.Lib.Wei.Eval
-import LscV2.Lib.Wei.Lower
+import LscV2.Lib.Wei.Optimize
