v2/LscV2/Prelude.lean
@@ -1,11 +1,11 @@
 import LscV2.Types
 import LscV2.Arithmetic
 import LscV2.Lib.Wei
-import LscV2.AST
-import LscV2.Eval
-import LscV2.Checks
-import LscV2.Syntax
-import LscV2.Contract
+import LscV2.Lang.AST
+import LscV2.Lang.Eval
+import LscV2.Lang.Checks
+import LscV2.Lang.Syntax
+import LscV2.Lang.Contract
 import LscV2.Compile.Yul
 
 namespace LscV2
