v2/LscV2/Selectors.lean
@@ -1,4 +1,4 @@
-import LscV2.AST
+import LscV2.Lang.AST
 
 namespace LscV2
 
