v2/examples/counter/test/CounterTheorem.lean
@@ -1,6 +1,6 @@
 import Counter
 import CounterProofs
-import LscV2.Eval
+import LscV2.Lang.Eval
 
 open LscV2 Counter
 
